Examples/WaitFreeStack.v
@@ -1,0 +1,680 @@
+From LHL.Core Require Import
+  ProgramRules
+  Program
+  LogicFacts
+  SingConds
+  Program
+  ProgramRules
+  ProgramFacts
+  Traces
+  Tensor
+  Logic
+  Specs
+  VisPoss.
+
+From LHL.Util Require Import
+  TransUtil
+  Tactics
+  Util.
+
+From LHL.Examples Require Import
+  CASSpec
+  MemSpec
+  WaitFreeStackSpec.
+Import WriteRacyMem.
+
+From Coq Require Import
+  Lists.List
+  Logic.FunctionalExtensionality
+  Logic.PropExtensionality.
+Import ListNotations.
+
+Require Import Coq.Program.Equality.
+
+Unset Printing Records.
+
+Definition E A :=
+  CASSig (Addr) |+| MemSig (A * option Addr).
+
+Definition F A := WaitFreeStackSig A.
+
+Definition wfpush {A} (v : A) : Prog (E A) (StkRet unit) :=
+  old <- call Get;
+  new <- call MAlloc;
+  call (MWrite new (v, old));;
+  b <- call (CAS old (Some new));
+  if b : bool then ret (PASS tt) else ret FAIL.
+
+Definition wfpop {A} : Prog (E A) (StkRet (option A)) :=
+  old <- call Get;
+  match old : option Addr with
+  | Some addr =>
+      head <- call (MRead addr);
+      b <- call (CAS old (snd head));
+      if b : bool then ret (PASS (Some (fst head))) else ret FAIL
+  | None => ret (PASS None)
+  end.
+
+Definition WFStack A : Impl (E A) (F A) :=
+  fun _ m => match m with
+  | WFPush v => wfpush v
+  | WFPop => wfpop
+  end.
+
+Module AtomicWFStackProof.
+  Import AtomicWFStack.
+  Parameter T:nat.
+  Parameter A:Type.
+
+  Definition VE : Spec T (E A) := tensorSpec casSpec memSpec.
+  Definition VF : Spec T (F A) := WFStackSpec.
+  
+  Definition Prec := SPrec VE VF.
+  Definition Relt := SRelt VE VF.
+  Definition Post R := R -> SRelt VE VF.
+
+  Definition ISt := InterState (F A) VE.
+
+  Definition casSt (s:ISt) := (LState (snd s)).
+  Definition memSt (s:ISt) := (RState (snd s)).
+  Notation casEv e := (inl e).
+  Notation memEv e := (inr e).
+
+  Inductive list_seg (s:option Heap) : option Addr (*head*) -> option Addr (*tail*) -> list A (*list value*) -> Prop :=
+  | ListSegNil l h :
+      s = Some h ->
+      list_seg s l l nil
+  | ListSegCons h l l1 l2 l3 v vs:
+      l1 = Some l ->
+      s = Some h ->
+      h l = Some (v, l2) ->
+      list_seg s l2 l3 vs ->
+      list_seg s l1 l3 (v :: vs)
+  .
+  
+  Definition eval_stack_und (s:ISt) (vs : list A) : Prop :=
+    list_seg (eval_heap (memSt s)) (eval_cas (casSt s)) None vs.
+  
+  Section EvalStackLemma.
+    Lemma EvalStackSameUndState: forall (s1 s2:ISt) vs,
+      snd s1 = snd s2 ->
+      eval_stack_und s1 vs ->
+      eval_stack_und s2 vs.
+    Proof.
+      destruct s1, s2.
+      unfold eval_stack_und.
+      unfold casSt, memSt.
+      simpl. intros. subst. auto.
+    Qed.
+
+    
+    Lemma ListSegFrame: forall h l v hd tl vs,
+      h l = None ->
+      list_seg (Some h) hd tl vs ->
+      list_seg (Some (heap_update l v h)) hd tl vs.
+    Proof.
+      intros.
+      remember (Some h) as s.
+      generalize dependent h.
+      induction H0; intros.
+      - eapply ListSegNil; eauto.
+      - specialize (IHlist_seg _ H3 Heqs).
+        econstructor; [|reflexivity| |apply IHlist_seg];
+        eauto. unfold heap_update.
+        destruct (Nat.eqb l l0) eqn:eq.
+        + apply EqNat.beq_nat_true_stt in eq. congruence.
+        + rewrite H0 in Heqs; inversion Heqs; subst.
+          rewrite H1; auto.
+    Qed.
+  End EvalStackLemma.
+  
+
+  Notation IStep s i e t :=
+    (InterStep (WFStack _) s (i, UEvent (Some e)) t).
+
+  Variant WFSTran : Name T -> Relt :=
+    | StkInvoke i s1 s2 ρ1 ρ2:
+      InvokeAny (WFStack A) i s1 (eq ρ1) s2 (eq ρ2) ->
+      WFSTran i s1 ρ1 s2 ρ2
+    | StkReturn i s1 s2 ρ1 ρ2:
+      ReturnAny (WFStack A) i s1 (eq ρ1) s2 (eq ρ2) ->
+      WFSTran i s1 ρ1 s2 ρ2
+    (* get *)
+    | StkGetCall i s1 ρ s2:
+      IStep s1 i (CallEv (casEv Get)) s2 ->
+      WFSTran i s1 ρ s2 ρ
+    | StkGetRetId i s1 ρ s2 old:
+      IStep s1 i (RetEv (casEv Get) old) s2 ->
+      WFSTran i s1 ρ s2 ρ
+    | StkGetRetEmp i s1 ρ1 s2 ρ2:
+      IStep s1 i (RetEv (casEv Get) None) s2 ->
+      VisPossSteps ρ1 [(i, CallEv WFPop); (i, RetEv WFPop (PASS None))] ρ2 ->
+      WFSTran i s1 ρ1 s2 ρ2
+    (* alloc *)
+    | StkAllocCall i s1 ρ s2:
+      IStep s1 i (CallEv (memEv MAlloc)) s2 ->
+      WFSTran i s1 ρ s2 ρ
+    | StkAllocRet i s1 ρ s2 new:
+      IStep s1 i (RetEv (memEv MAlloc) new) s2 ->
+      WFSTran i s1 ρ s2 ρ
+    (* write *)
+    | StkWriteCall i s1 ρ s2 new data:
+      IStep s1 i (CallEv (memEv (MWrite new data))) s2 ->
+      WFSTran i s1 ρ s2 ρ
+    | StkWriteRet i s1 ρ s2 new data:
+      IStep s1 i (RetEv (memEv (MWrite new data)) tt) s2 ->
+      WFSTran i s1 ρ s2 ρ
+    (* read *)
+    | StkReadCall i s1 ρ s2 addr:
+      IStep s1 i (CallEv (memEv (MRead addr))) s2 ->
+      WFSTran i s1 ρ s2 ρ
+    | StkReadRet i s1 ρ s2 addr v:
+      IStep s1 i (RetEv (memEv (MRead addr)) v) s2 ->
+      WFSTran i s1 ρ s2 ρ
+    (* cas *)
+    | StkCASCall i s1 ρ s2 old new:
+      IStep s1 i (CallEv (casEv (CAS old new))) s2 ->
+      WFSTran i s1 ρ s2 ρ
+    | StkCASRetPushPass i s1 s2 ρ1 ρ2 old new v:
+      (* TODO: side condition: new points to (v, old) *)
+      IStep s1 i (RetEv (casEv (CAS old new)) true) s2 ->
+      VisPossSteps ρ1 [(i, CallEv (WFPush v)); (i, RetEv (WFPush v) (PASS tt))] ρ2 ->
+      WFSTran i s1 ρ1 s2 ρ2
+    | StkCASRetPushFail i s1 s2 ρ1 ρ2 old new v:
+      IStep s1 i (RetEv (casEv (CAS old new)) false) s2 ->
+      VisPossSteps ρ1 [(i, CallEv (WFPush v)); (i, RetEv (WFPush v) FAIL)] ρ2 ->
+      WFSTran i s1 ρ1 s2 ρ2
+    | StkCASRetPopPass i s1 s2 ρ1 ρ2 old new v:
+      (* TODO: side condition: old points to (v, new) *)
+      IStep s1 i (RetEv (casEv (CAS old new)) true) s2 ->
+      VisPossSteps ρ1 [(i, CallEv WFPop); (i, RetEv WFPop (PASS (Some v)))] ρ2 ->
+      WFSTran i s1 ρ1 s2 ρ2
+    | StkCASRetPopFail i s1 s2 ρ1 ρ2 old new:
+      IStep s1 i (RetEv (casEv (CAS old new)) false) s2 ->
+      VisPossSteps ρ1 [(i, CallEv WFPop); (i, RetEv WFPop FAIL)] ρ2 ->
+      WFSTran i s1 ρ1 s2 ρ2
+  .
+
+  Definition Guar (i : Name T) : Relt := WFSTran i.
+
+  Definition Rely (i : Name T) : Relt :=
+    SRTC (fun s x t y => exists j, i <> j /\ WFSTran j s x t y).
+
+  Record Inv (s : ISt) (x : Poss VF) := {
+    stack_consistent :
+      eval_stack_und s (eval_stack (PState x))
+  }.
+
+  Record Ready (i : Name T) (s : ISt) (x : Poss VF) := {
+    ready_inv : Inv s x;
+  }.
+
+  Record ReadyDone (i : Name T) {R} (m : F A R) (r : R) (s : ISt) (x : Poss VF) := {
+    done_ready : Ready i s x;
+    ready_done : Done i m r x;
+  }.
+
+  Section SideConditions.
+    Lemma RelyReflexive:
+      forall (i : Name T) (s : @InterState T (E A) (F A) VE) (ρ : @PossSet T (F A) VF), @LiftSRelt T (E A) (F A) VE VF (Rely i) s ρ s ρ.
+    Proof.
+      intros.
+      eexists. subst.
+      split. easy.
+      constructor.
+    Qed.
+
+    Lemma RelyClosed:
+      forall i : Name T,
+      @sub (@Logic.Relt T (E A) (F A) VE VF) (@subRelt T (E A) (F A) VE VF)
+        (@ReltCompose T (E A) (F A) VE VF (@LiftSRelt T (E A) (F A) VE VF (Rely i))
+          (@LiftSRelt T (E A) (F A) VE VF (Rely i))) (@LiftSRelt T (E A) (F A) VE VF (Rely i)).
+    Proof.
+      unfold sub, subRelt, LiftSRelt.
+      intros. psimpl.
+      specialize (H x eq_refl). psimpl.
+      specialize (H1 x2 eq_refl). psimpl.
+      eexists. split. easy.
+      eapply srtcTrans.
+      psplit. exact H0. easy.
+    Qed.
+
+    Lemma GuarInRely:
+      forall (i j : Name T) (_ : not (@eq (Name T) i j)),
+      @sub (@Logic.Relt T (E A) (F A) VE VF) (@subRelt T (E A) (F A) VE VF)
+        (@LiftSRelt T (E A) (F A) VE VF (Guar i)) (@LiftSRelt T (E A) (F A) VE VF (Rely j)).
+    Proof.
+      unfold sub, subRelt, LiftSRelt.
+      intros. psimpl.
+      specialize (H0 x eq_refl). psimpl.
+      eexists. split. easy.
+      econstructor.
+      2: constructor.
+      now exists i.
+    Qed.
+
+    Lemma Invoke_pres_single {R} :
+      forall (m : F A R) i s ρ t σs,
+      TInvoke (VE:= VE) (VF:= VF) (WFStack A) i R m s (eq ρ) t σs ->
+      exists σ, σs = eq σ.
+    Proof.
+      intros.
+      unfold TInvoke in H. psimpl.
+      exists (invPoss i ρ m).
+      set_ext σ. split; intros; destruct_all; subst.
+      {
+        unfold TIdle in H. destruct_all.
+        specialize (H2 x eq_refl). destruct_all.
+        destruct x, σ. unfold invPoss. cbn in *.
+        f_equal; try easy.
+        extensionality j. dec_eq_nats i j.
+        rewrite eqb_id. easy.
+        rewrite eqb_nid, H6; easy.
+        extensionality j. dec_eq_nats i j.
+        rewrite eqb_id. easy.
+        rewrite eqb_nid, H7; easy.
+      }
+      {
+        cbn. rewrite eqb_id. exists ρ.
+        repeat split; (easy || apply differ_pointwise_trivial).
+      }
+    Qed.
+
+    Lemma InvokeInRely:
+      forall (i j : Name T) (_ : not (@eq (Name T) i j)),
+      @sub (@Logic.Relt T (E A) (F A) VE VF) (@subRelt T (E A) (F A) VE VF)
+        (@InvokeAny T (E A) (F A) VE VF (WFStack A) i)
+        (@LiftSRelt T (E A) (F A) VE VF (Rely j)).
+    Proof.
+      unfold sub, subRelt, LiftSRelt.
+      intros. psimpl.
+      assert (exists x, σ = eq x).
+      {
+        unfold InvokeAny in H0. psimpl.
+        eapply Invoke_pres_single.
+        exact H0.
+      }
+      psimpl.
+      eexists. split. easy.
+      econstructor. 2: constructor.
+      exists i. split. easy.
+      apply StkInvoke. easy.
+    Qed.
+
+    Lemma Return_pres_single {R} :
+      forall (m : F A R) v i s ρ t σs,
+      TReturn (VE:= VE) (VF:= VF) (WFStack A) i m v s (eq ρ) t σs ->
+      exists σ, σs = eq σ.
+    Proof.
+      intros.
+      unfold TReturn, mapRetPoss in H. psimpl.
+      exists (retPoss i ρ).
+      set_ext σ. split; intros; destruct_all; subst.
+      {
+        unfold retPoss. destruct x, σ. cbn in *.
+        f_equal. easy.
+        extensionality j. dec_eq_nats i j.
+        rewrite eqb_id. easy.
+        rewrite eqb_nid, H7; easy.
+        extensionality j. dec_eq_nats i j.
+        rewrite eqb_id. easy.
+        rewrite eqb_nid, H8; easy.
+      }
+      {
+        cbn. rewrite eqb_id. exists ρ.
+        destruct H0. ddestruct H0. cbn in *.
+        symmetry in x0. apply H in x0.
+        specialize (x0 ρ eq_refl).
+        repeat split; (easy || apply differ_pointwise_trivial).
+      }
+    Qed.
+
+    Lemma ReturnInRely:
+      forall (i j : Name T) (_ : not (@eq (Name T) i j)),
+      @sub (@Logic.Relt T (E A) (F A) VE VF) (@subRelt T (E A) (F A) VE VF)
+        (@ReturnAny T (E A) (F A) VE VF (WFStack A) i)
+        (@LiftSRelt T (E A) (F A) VE VF (Rely j)).
+    Proof.
+      unfold sub, subRelt, LiftSRelt.
+      intros. psimpl.
+      assert (exists x, σ = eq x).
+      {
+        unfold ReturnAny in H0. psimpl.
+        eapply Return_pres_single.
+        exact H0.
+      }
+      psimpl.
+      eexists. split. easy.
+      econstructor. 2: constructor.
+      exists i. split. easy.
+      apply StkReturn. easy.
+    Qed.
+
+    Lemma InitialReady:
+      forall (i : Name T) (A0 : Type) (_ : F A A0),
+      @LiftSPrec T (E A) (F A) VE VF (Ready i)
+        (@pair (ThreadsSt T (E A) (F A)) (@State T (E A) VE) (@allIdle T (E A) (F A))
+          (@Init T (E A) VE)) (@eq (@Poss T (F A) VF) (@initPoss T (F A) VF)).
+    Proof.
+      unfold LiftSPrec.
+      intros. eexists.
+      split. easy.
+      constructor.
+      {
+        constructor. simpl eval_stack.
+        unfold eval_stack_und.
+        simpl. eapply ListSegNil. eauto.
+      }
+    Qed.
+    
+    Ltac begin_stable :=
+      unfold Stable, stablePost, stableRelt, stablePrec, sub, subRelt, subPrec;
+      unfold SStable, stableSRelt, stableSPrec, ssub, subSRelt, subSPrec;
+      unfold ReltToPrec, LiftSPrec, LiftSRelt;
+      intros; psimpl.
+
+    Lemma sing_elem {A} {P : A -> Prop} :
+      forall x : A,
+      eq x = P ->
+      P x.
+    Proof.
+    intros. now rewrite <- H.
+    Qed.
+
+    Ltac forward_istep_cas stack_consistent0 :=
+    match goal with
+      | H : IStep ?s1 _ _ ?s2 |- _ =>
+        destruct H as [_ [H ?]]; psimpl;
+        unfold eval_stack_und, casSt, memSt in *;
+        inversion H; subst; clear H;
+        match goal with
+        | Hs1 : _ = LState (snd s1),
+          Hs2R : _ = RState (snd s2),
+          Hs2L : _ = LState (snd s2) |- _ =>
+          setoid_rewrite <- Hs2R;
+          setoid_rewrite <- Hs2L;
+          setoid_rewrite <- Hs1 in stack_consistent0
+        end
+      end.
+
+    Ltac forward_pstep p1 p2 :=
+      match goal with
+      | H : VisPossStep p1 _ p2 |- _ =>
+        inversion H; subst; clear H;
+        match goal with
+        | H1 : Step _ (PState p1) _ (PState p2) |- _ =>
+          inversion H1; subst; clear H1
+        end
+      end.
+    
+    Ltac simp_eqs :=
+      do 10 try (
+        lazymatch goal with
+        | [ H1 : ?y = ?x, H2 : ?z = ?x |- _ ] =>
+          rewrite <- H2 in H1 at 1;
+          ddestruct H1
+        | [ H1 : ?x = ?y, H2 : ?z = ?x |- _ ] =>
+          rewrite H1 in H2;
+          ddestruct H2
+        | [ H1 : ?x = ?y, H2 : ?y = ?z |- _ ] =>
+          rewrite H2 in H1 at 1;
+          ddestruct H1
+        | [ H1 : ?x = ?y, H2 : ?z = ?y |- _ ] =>
+          rewrite <- H2 in H1 at 1;
+          ddestruct H1
+        | [ H : existT ?F ?A ?x = existT ?F ?A ?y |- _ ] =>
+          ddestruct H
+        end
+      ).
+
+    Lemma InvStable: forall i (s1 s2:InterState (F A) VE) p1 p2,
+      Ready i s1 p1 ->
+      (exists j, i <> j /\ WFSTran j s1 p1 s2 p2) ->
+      Ready i s2 p2.
+    Proof.
+      intros.
+      destruct H0 as [j [? ?]].
+      constructor; constructor.
+      inversion_clear H.
+      inversion_clear ready_inv0.
+      inversion H1; subst; clear H1;
+      (* irrelevant cas events *)
+      try (forward_istep_cas stack_consistent0; now auto).
+      (* invoke any *)
+      {
+        unfold InvokeAny, TInvoke, TIdle in H.
+        psimpl. apply sing_elem in H3. psimpl.
+        rewrite H5.
+        eapply EvalStackSameUndState; eauto.
+      }
+      (* return any *)
+      {
+        unfold ReturnAny, TReturn, mapRetPoss in H.
+        psimpl. apply sing_elem in H3. psimpl.
+        rewrite H10.
+        eapply EvalStackSameUndState; eauto.
+      }
+      (* fail pop *)
+      {
+        forward_istep_cas stack_consistent0.
+        inversion H2; subst; clear H2.
+        inversion H16; subst; clear H16.
+        inversion H19; subst; clear H19.
+        forward_pstep p1 y.
+        setoid_rewrite <- H2 in stack_consistent0.
+        forward_pstep y p2;
+        simp_eqs; simpl in *; auto.
+      }
+      (* malloc call *)
+      {
+        destruct H as [_ [H ?]]; psimpl;
+        unfold eval_stack_und, casSt, memSt in *;
+        inversion H; subst; clear H;
+        match goal with
+        | Hs1 : _ = RState (snd s1) |- _ =>
+          setoid_rewrite <- Hs1 in stack_consistent0
+        end; simpl in *;
+        [|inversion stack_consistent0; congruence].
+        setoid_rewrite <- H4.
+        setoid_rewrite <- H8.
+        auto.
+      }
+      (* malloc ret *)
+      {
+        destruct H as [_ [H ?]]; psimpl;
+        unfold eval_stack_und, casSt, memSt in *;
+        inversion H; subst; clear H;
+        match goal with
+        | Hs1 : _ = RState (snd s1) |- _ =>
+          setoid_rewrite <- Hs1 in stack_consistent0
+        end; simpl in *;
+        [|inversion stack_consistent0; congruence
+         |inversion stack_consistent0; congruence].
+        setoid_rewrite <- H4.
+        setoid_rewrite <- H9.
+        simpl in *.
+        apply ListSegFrame; auto.
+      }
+      {
+        destruct H as [_ [H ?]]; psimpl;
+        unfold eval_stack_und, casSt, memSt in *;
+        inversion H; subst; clear H.
+        - (*provable*)
+          admit.
+        - (*unprovable*)
+          (* different threads should not be able to write to the same location *)
+          (* TODO: add extra field in mem state to record TID that allocates each location, and ensure in the rely that each thread only write to the one it allocates *)
+          admit.
+        - (*provable*)
+          admit.
+      }
+
+        2:{
+          
+          setoid_rewrite <- H6 in stack_consistent0.
+        match goal with
+        | H : IStep ?s1 _ _ ?s2 |- _ =>
+          destruct H as [_ [H ?]]; psimpl;
+          unfold eval_stack_und, casSt, memSt in *;
+          inversion H; subst; clear H
+        end.
+          match goal with
+          | Hs1 : _ = LState (snd s1),
+            Hs2R : _ = RState (snd s2),
+            Hs2L : _ = LState (snd s2) |- _ =>
+            setoid_rewrite <- Hs2R;
+            setoid_rewrite <- Hs2L;
+            setoid_rewrite <- Hs1 in stack_consistent0
+          end
+        end.
+      }
+
+
+    Lemma InitialStable:
+      forall (i : Name T) (A0 : Type) (_ : F A A0),
+      @Stable T (E A) (F A) VE VF (@Logic.Prec T (E A) (F A) VE VF)
+        (@stablePrec T (E A) (F A) VE VF) (@LiftSRelt T (E A) (F A) VE VF (Rely i))
+        (@LiftSPrec T (E A) (F A) VE VF (Ready i)).
+    Proof.
+      begin_stable.
+      specialize (H0 x1 eq_refl). psimpl.
+      eexists. split. easy.
+      induction H0; auto; clear H0.
+      apply IHSRTC; clear IHSRTC.
+      clear - H H1.
+      constructor; constructor.
+      inversion_clear H1.
+      inversion_clear ready_inv0.
+      
+
+      destruct H as [j [? ?]].
+
+          (* {
+            
+          }
+          {
+            
+          }
+          {
+            unfold sub, subRelt, LiftSRelt.
+            intros. psimpl.
+            assert (exists x, σ = eq x).
+            {
+              unfold ReturnAny in H0. psimpl.
+              eapply Return_pres_single.
+              exact H0.
+            }
+            psimpl.
+            eexists. split. easy.
+            econstructor. 2: constructor.
+            exists i. split. easy.
+            apply StkReturn. easy.
+          } *)
+
+
+    (* Lemma RelyReflective :
+    forall (i : Name T) (s : InterState (F A) VE) (ρ : PossSet VF), Rely i s ρ s ρ.
+    2/10
+    forall i : Name T, Rely i ->> Rely i ==> Rely i
+    3/10
+    forall i j : Name T, i <> j -> Guar i ==> Rely j
+    4/10
+    forall i j : Name T, i <> j -> InvokeAny (WFStack A) i ==> Rely j
+    5/10
+    forall i j : Name T, i <> j -> ReturnAny (WFStack A) i ==> Rely j
+    6/10
+    forall (i : Name T) (A0 : Type), F A A0 -> Ready i (allIdle, Init VE) (eq initPoss)
+    7/10
+    forall (i : Name T) (A0 : Type), F A A0 -> Stable (Rely i) (Ready i) *)
+
+  End SideConditions.
+  
+
+  Theorem WFStackCorrect:
+    VerifyImpl VE VF
+    (fun i => LiftSRelt (Rely i))
+    (fun i => LiftSRelt (Guar i))
+    (fun i _ _ => LiftSPrec (Ready i))
+    (WFStack A)
+    (fun i _ m r _ _ => LiftSPrec (ReadyDone i m r))
+    (TReturn (WFStack A)).
+  Proof.
+    constructor.
+    7:{
+    Set Printing All.
+  Qed.
+End AtomicWFStackProof.
+
+
+
+
+
+Record Complete {T A} (i : Name T) (v : option A)
+  (s : InterState (F A) (VE T A)) (x : Poss (VF T A))
+:= {
+  comp_inv : Inv s x;
+  comp_pres : contains (i, v) (pendSet s);
+  comp_emp : doneSet s = {}
+}.
+
+Record ReadyWaiting {T A} (i : Name T) {R} (m : F A R)
+  (s : InterState (F A) (VE T A)) (x : Poss (VF T A))
+:= {
+  wait_ready : Ready i s x;
+  ready_wait : Waiting i m x
+}.
+
+Record ReadyDone {T A} (i : Name T) {R} (m : F A R) (r : R)
+  (s : InterState (F A) (VE T A)) (x : Poss (VF T A))
+:= {
+  done_ready : Ready i s x;
+  ready_done : Done i m r x;
+}.
+
+From Equations Require Import Equations.
+
+Equations rde_prop {T A R}
+  (s : InterState (F A) (VE T A))
+  (i : Name T) (m : F A R) (r : R) : Prop :=
+rde_prop s i (Push v) _ :=
+  exists j, exchSt s = ExchDef {j => None} {i => Some v};
+rde_prop s i Pop v :=
+  exists j, exchSt s = ExchDef {j => v} {i => None}.
+
+Record ReadyDoneExch {T A} (i : Name T) {R} (m : F A R) (r : R)
+  (s : InterState (F A) (VE T A)) (x : Poss (VF T A))
+:= {
+  dexch_ready : ReadyDone i m r s x;
+  ready_proper : rde_prop s i m r
+}.
+
+Record Conflicted {T A} (i : Name T) {R} (m : F A R)
+  (s : InterState (F A) (VE T A)) (x : Poss (VF T A))
+:= {
+  wexch_ready : ReadyWaiting i m s x;
+  ready_improper :
+    match m with
+    | Push v => exists j w, exchSt s = ExchDef {j => Some w} {i => Some v}
+    | Pop => exists j, exchSt s = ExchDef {j => None} {i => None}
+    end
+}.
+
+
+Theorem EBStackCorrect T A :
+  VerifyImpl (VE T A) (VF T A)
+  (fun i => LiftSRelt (Rely i))
+  (fun i => LiftSRelt (Guar i))
+  (fun i _ _ => LiftSPrec (Ready i))
+  (EBStack A)
+  (fun i _ m r _ _ => LiftSPrec (ReadyDone i m r))
+  (TReturn (EBStack A)).
+Proof.
+Qed.
+
+Require Import LHL.Core.Linearizability.
+
+Theorem EBStackLin T A :
+  Lin (overObj (VE T A :> EBStack A)) (VF T A).
+eapply soundness.
+apply EBStackCorrect.
+Qed.
